add impl.delete_avl_aux0
a bit messy: will be fixed

Impl.fst
@@ -914,8 +914,8 @@ let rec insert_avl2 (#a: Type)
   )
 #pop-options
 
-#push-options "--fuel 1 --ifuel 1 --z3rlimit 50"
-let rec remove_leftmost (#a: Type0) (cmp:cmp a) (ptr: t a)
+#push-options "--fuel 1 --ifuel 1 --z3rlimit 100"
+let rec remove_leftmost_avl (#a: Type0) (cmp:cmp a) (ptr: t a)
   : Steel (t a & a)
   (linked_tree ptr)
   (fun r -> linked_tree (fst r))
@@ -925,10 +925,14 @@ let rec remove_leftmost (#a: Type0) (cmp:cmp a) (ptr: t a)
   (ensures fun h0 r h1 ->
     Spec.Node? (v_linked_tree ptr h0) /\
     Spec.is_avl (convert cmp) (v_linked_tree ptr h0) /\
-    (let r2 = Spec.remove_leftmost
-      (convert cmp) (v_linked_tree ptr h0) in
-    v_linked_tree (fst r) h1 == fst r2 /\
-    I.eq (cmp (snd r) (snd r2)) I.zero))
+    v_linked_tree (fst r) h1
+    == fst (Spec.remove_leftmost_avl
+      (convert cmp) (v_linked_tree ptr h0)) /\
+    snd r == snd (Spec.remove_leftmost_avl
+      (convert cmp) (v_linked_tree ptr h0)) /\
+    Spec.size_of_tree (v_linked_tree (fst r) h1)
+    == Spec.size_of_tree (v_linked_tree ptr h0) - 1 /\
+    Spec.is_avl (convert cmp) (v_linked_tree ptr h0))
   =
   (**) node_is_not_null ptr;
   (**) let node = unpack_tree ptr in
@@ -940,7 +944,7 @@ let rec remove_leftmost (#a: Type0) (cmp:cmp a) (ptr: t a)
     return (get_right node, data)
   ) else (
     (**) not_null_is_node (get_left node);
-    let r0 = remove_leftmost cmp (get_left node) in
+    let r0 = remove_leftmost_avl cmp (get_left node) in
     let old_size = read (get_size node) in
     write (get_size node) (U.sub old_size one);
     let new_node = mk_node (get_data node)
@@ -953,7 +957,12 @@ let rec remove_leftmost (#a: Type0) (cmp:cmp a) (ptr: t a)
   )
 #pop-options
 
-#push-options "--fuel 1 --ifuel 1 --z3rlimit 50"
+let cdata = Spec.cdata
+let cleft = Spec.cleft
+let cright = Spec.cright
+
+#push-options "--fuel 1 --ifuel 1 --z3rlimit 100"
+//#push-options "--fuel 1 --ifuel 1"
 let delete_avl_aux0 (#a: Type0)
   (cmp:cmp a) (ptr: t a) (data_to_rm: a)
   : Steel (t a)
@@ -970,28 +979,35 @@ let delete_avl_aux0 (#a: Type0)
     (v_linked_tree ptr' h1
     == Spec.delete_avl_aux0
       (convert cmp) (v_linked_tree ptr h0) data_to_rm) /\
-    Spec.is_avl (convert cmp) (v_linked_tree ptr' h1))
+    Spec.size_of_tree (v_linked_tree ptr' h1)
+    == Spec.size_of_tree (v_linked_tree ptr h0) - 1)
   =
+  let h00 = get () in
   (**) node_is_not_null ptr;
   (**) let node = unpack_tree ptr in
   if is_null_t (get_left node) && is_null_t (get_right node) then (
+    //sladmit (); admit ();
     elim_linked_tree_leaf (get_left node);
     free (get_size node);
     free ptr;
     return (get_right node)
   ) else if is_null_t (get_right node) then (
+    //sladmit (); admit ();
     elim_linked_tree_leaf (get_right node);
     free (get_size node);
     free ptr;
     return (get_left node)
   ) else if is_null_t (get_left node) then (
+    //sladmit (); admit ();
     elim_linked_tree_leaf (get_left node);
     free (get_size node);
     free ptr;
     return (get_right node)
   ) else (
+    //let h01 = get () in
     let right_node = unpack_tree (get_right node) in
     if is_null_t (get_left right_node) then (
+      //sladmit (); admit ();
       let y = get_data right_node in
       elim_linked_tree_leaf (get_left right_node);
       free (get_size right_node);
@@ -1003,25 +1019,171 @@ let delete_avl_aux0 (#a: Type0)
       write ptr new_node;
       pack_tree ptr
         (get_left node) (get_right right_node) (get_size node);
-      rebalance_avl ptr
+      return ptr
     ) else (
       pack_tree (get_right node)
         (get_left right_node) (get_right right_node)
         (get_size right_node);
-      let result = remove_leftmost cmp (get_right node) in
+      //let h02 = get () in
+      //assert (
+      //  v_linked_tree (get_right node) h01
+      //  ==
+      //  v_linked_tree (get_right node) h02
+      //);
+      //assert (
+      //  v_linked_tree (get_left node) h01
+      //  ==
+      //  v_linked_tree (get_left node) h02
+      //);
+      //admit (); //sladmit ();
+      let h0 = get () in
+      //assume (Spec.is_avl (convert cmp) (v_linked_tree (get_right node) h0));
+      //assume (Spec.Node? (v_linked_tree (get_right node) h0));
+      let result_spec = hide (Spec.remove_leftmost_avl
+        (convert cmp) (v_linked_tree (get_right node) h0)) in
+      let result = remove_leftmost_avl cmp (get_right node) in
+      assert (snd result == snd (reveal result_spec));
+      //admit ();
+      //assume (v_linked_tree (fst result) h1 == fst (reveal result_spec));
+            //let h0 = get () in
+      //let h1 = get () in
+      //assert (let r2 = Spec.remove_leftmost
+      //(convert cmp) (v_linked_tree (get_right node) h0) in
+      //v_linked_tree (fst result) h1 == fst r2 /\
+    //I.eq (cmp (snd result) (snd r2)) I.zero);
+      //admit ();
       let sz = read (get_size node) in
       write (get_size node) (U.sub sz one);
+      let h1 = get () in
+      assert (
+       Spec.size_of_tree (v_linked_tree (fst result) h1)
+       ==
+       Spec.size_of_tree (v_linked_tree (get_right node) h0) - 1);
+      assert (U.v (sel (get_size node) h0)
+      == Spec.size_of_tree (v_linked_tree (get_left node) h0)
+       + Spec.size_of_tree (v_linked_tree (get_right node) h0)
+       + 1);
+      assert (U.v (sel (get_size node) h0)
+      == U.v (sel (get_size node) h1) + 1);
+
       let new_node = mk_node (snd result)
-        (get_right node) (fst result) (get_size node) in
+        (get_left node) (fst result) (get_size node) in
       write ptr new_node;
-      // @AF: this sladmit should be removed
-      sladmit ();
+      let h = get () in
+      assert (U.v (sel (get_size node) h)
+      == Spec.size_of_tree (v_linked_tree (get_left node) h)
+       + Spec.size_of_tree (v_linked_tree (fst result) h)
+       + 1);
+      //admit ();
       pack_tree ptr
-        (get_right node) (fst result) (get_size node);
-      rebalance_avl ptr
+        (get_left node) (fst result) (get_size node);
+      let orig = hide (v_linked_tree ptr h00) in
+      let result_spec = hide (Spec.delete_avl_aux0
+        (convert cmp) (reveal orig) data_to_rm) in
+      let h = get () in
+      let result = hide (v_linked_tree ptr h) in
+      assert (cdata (reveal result) == cdata (reveal result_spec));
+      assert (cleft (reveal result) == cleft (reveal result_spec));
+      assert (cright (reveal result) == cright (reveal result_spec));
+      return ptr
     )
   )
 #pop-options
+
+let u_of_bool (b:bool) : x:U.t{U.v x = Spec.int_of_bool b}
+= match b with
+| true -> one
+| false -> zero
+
+#push-options "--fuel 1 --ifuel 1"
+let dincr
+  (b: bool)
+  (ptr: ref U.t)
+  : Steel unit
+  (vptr ptr) (fun _ -> vptr ptr)
+  (requires fun h0 ->
+    U.gt (sel ptr h0) zero)
+  (ensures fun h0 _ h1 ->
+    (let old_value = sel ptr h0 in
+    U.gt (sel ptr h0) zero /\
+    sel ptr h1 = U.sub old_value (u_of_bool b)))
+  =
+  if b then (
+    let old_value = read ptr in
+    write ptr (U.sub old_value one);
+    return ()
+  ) else (
+    return ()
+  )
+
+
+#push-options "--fuel 1 --ifuel 1 --z3rlimit 100"
+let rec delete_avl_aux (#a: Type0)
+  (cmp:cmp  a) (ptr: t a) (data_to_rm: a)
+  : Steel (t a & bool)
+  (linked_tree ptr)
+  (fun r -> linked_tree (fst r))
+  (requires fun h0 ->
+    Spec.is_avl (convert cmp) (v_linked_tree ptr h0))
+  (ensures fun h0 r h1 ->
+    Spec.is_avl (convert cmp) (v_linked_tree ptr h0) /\
+    (let r2 = Spec.delete_avl_aux
+      (convert cmp) (v_linked_tree ptr h0) data_to_rm in
+    v_linked_tree (fst r) h1 == fst r2 /\
+    snd r == snd r2) /\
+    Spec.is_avl (convert cmp) (v_linked_tree (fst r) h1))
+  =
+  if is_null_t #a ptr then (
+    (**) null_is_leaf ptr;
+    let h = get () in
+    return (ptr, false)
+  ) else (
+    (**) let node = unpack_tree ptr in
+    let delta = cmp data_to_rm (get_data node) in
+    if I.lt delta I.zero then (
+      let h0 = get () in
+      let result = delete_avl_aux cmp (get_left node) data_to_rm in
+      let h1 = get () in
+      dincr (snd result) (get_size node);
+      let h1 = get () in
+      assert (
+      U.v (sel (get_size node) h1)
+      ==
+      U.v (sel (get_size node) h0)
+      - (Spec.int_of_bool (snd result))
+      );
+      let new_node = mk_node (get_data node)
+        (fst result) (get_right node) (get_size node) in
+      write ptr new_node;
+      pack_tree ptr
+        (fst result) (get_right node) (get_size node);
+      let ptr = rebalance_avl ptr in
+      return (ptr, snd result)
+    ) else if I.gt delta I.zero then (
+      let h0 = get () in
+      let result = delete_avl_aux cmp (get_right node) data_to_rm in
+      dincr (snd result) (get_size node);
+      let h1 = get () in
+      assert (
+      U.v (sel (get_size node) h1)
+      ==
+      U.v (sel (get_size node) h0)
+      - (Spec.int_of_bool (snd result))
+      );
+      let new_node = mk_node (get_data node)
+        (get_left node) (fst result) (get_size node) in
+      write ptr new_node;
+      pack_tree ptr
+        (get_left node) (fst result) (get_size node);
+      let ptr = rebalance_avl ptr in
+      return (ptr, snd result)
+    ) else (
+      pack_tree ptr
+        (get_left node) (get_right node) (get_size node);
+      let ptr = delete_avl_aux0 cmp ptr data_to_rm in
+      return (ptr, true)
+    )
+  )
 
 (*
 let rec delete_avl (#a: eqtype)
